\begin{theorem} \label{thm:multiplicative:rules}
  Let $a,b\in \Rplus$ and $\epsilon,\delta \in\Rplusnull$. We have

  \begin{enumerate}
    \item $\delta \le \epsilon \implies \ean[\delta]{a} \subseteq \ean[\epsilon]{a}$ 
    \item $\ean[\epsilon]{a} \cdot \ean[\delta]{b} = \ean[\epsilon+\delta]{a\cdot b}$
    \item $\ean[\epsilon]{\ean[\delta]{a}} = \ean[\epsilon+\delta]{a}$
    \item $\ean[\epsilon]{a} + \ean[\epsilon]{b} = \ean[\epsilon]{a+b}$
    \item $\ean[\epsilon]{a} = \an[\sinh(\epsilon)a]{\cosh(\epsilon)a}$
    \item $\ean[\epsilon]{a} \subseteq \an[\left(e^\epsilon-1\right)a]{a}$
    \item $\abs{\frac ab-1} \le \epsilon \implies a\in\ean[\epsilon]{b}$
  \end{enumerate}
\end{theorem}
