\chapter{Proofs for the tools of this thesis}

In this chapter I will prove the theorems I have stated in the chapter~\ref{chapter:tools} where I presented the needed tools for this thesis.

\section{Interval arithmetic}

\input{additive_rules}

\begin{proof} ~
  \begin{enumerate}
    \item Claim $\an[\epsilon]{a} + \an[\delta]{b} \subseteq \an[\epsilon+\delta]{a+b}$:

      \begin{align}
        x \in \an[\epsilon]{a} \land y \in \an[\delta]{b} & \implies a-\epsilon \le x \le a+\epsilon \land b-\delta \le y \le b+\delta \nl
        & \implies (a+b)-(\epsilon + \delta) \le x+y \le (a+b)+(\epsilon + \delta) \nl
        & \implies x+y \in \an[\epsilon+\delta]{a+b}
      \end{align}

      Claim $\an[\epsilon+\delta]{a+b} \subseteq \an[\epsilon]{a} + \an[\delta]{b}$: Let $f$ be the function $f: \an[\epsilon]{a} \times \an[\delta]{b} \to \R$ with $f(x,y) =x+y$ so that $\an[\epsilon]{a} + \an[\delta]{b}$ is the image of $f$. The function $f$ attains the maximum $a+b+\epsilon+\delta$ of the interval $\an[\epsilon+\delta]{a+b}$ for $(x,y) = \left(a+\epsilon,b+\delta\right)$ and its minimum $a+b-(\epsilon+\delta)$ for $(x,y)=\left(a-\epsilon,b-\delta\right)$. Because $f$ is continuous, $f$ attains each value between $a+b-(\epsilon+\delta)$ and $a+b+\epsilon+\delta$ and therefore each value of $\an[\epsilon+\delta]{a+b}$ (intermediate value theorem~\cite{wiki:intermediatevaluetheorem}).
    \item

      \begin{align}
        \an[\epsilon]{\an[\delta]{a}} & = \bigcup_{x\in \interval{a-\delta}{a+\delta}} \an[\epsilon]{x} = \bigcup_{x\in\interval{a-\delta}{a+\delta}} \bigcup_{y\in\interval{-\epsilon}{\epsilon}} \{x+y\} \nl
        &= \an[\delta]{a} + \an[\epsilon]{0} = \an[\epsilon+\delta]{a}
      \end{align}
 
    \item

      This follows directly from $-\abs{b} \le b \le \abs{b}$ because $b \in \{-\abs{b}, \abs{b}\}$.

    \item

      \begin{align}
        \an[\epsilon]{a+b} \subseteq \an[\epsilon]{a+\an[\abs{b}]{0}} = \an[\epsilon]{\an[\abs{b}]{a}} = \an[\epsilon+\abs{b}]{a}
      \end{align}

    \item
      Let $\lambda \ge 0$ and let $f_\lambda$ be the function $f_\lambda : \an[\epsilon]{a}\to\R:x\mapsto \lambda x$. $f_\lambda$ attains its maximum at $\lambda(a+\epsilon)$ and its minimum at $\lambda(a-\epsilon)$. Because $f_\lambda$ is continuous and $\an[\epsilon]{a}$ is connected, also $f_\lambda(\an[\epsilon]{a})$ is connected and therefore $f_\lambda$ attains all values between $\lambda(a-\epsilon)$ and $\lambda(a+\epsilon)$ (intermediate value theorem~\cite{wiki:intermediatevaluetheorem}). Thus

      \begin{align}
        f_\lambda\left(\an[\epsilon]{a}\right) = \interval{\lambda(a-\epsilon)}{\lambda(a+\epsilon} = \interval{\lambda a - \lambda \epsilon}{\lambda a+\lambda \epsilon} = \an[\lambda \epsilon]{\lambda a} = \an[\abs{\lambda}\cdot \epsilon]{\lambda a}
      \end{align}

      Let $\lambda < 0$ and $f_\lambda$ be as above. The maximum of this function is now $\lambda (a-\epsilon)$ and its minimum is $\lambda (a+\epsilon)$. Due to the intermediate value theorem~\cite{wiki:intermediatevaluetheorem} all values between $\lambda(a+\epsilon)$ and $\lambda(a-\epsilon)$ are attained by the function. So we have

      \begin{align}
        f_\lambda\left(\an[\lambda]{a}\right) = \interval{\lambda(a+\epsilon)}{\lambda(a-\epsilon)} = \interval{\lambda a -\abs{\lambda}\cdot \epsilon}{\lambda a + \abs{\lambda}\cdot \epsilon} = \an[\abs{\lambda}\cdot \epsilon]{\lambda a}
      \end{align}

 \end{enumerate}
\end{proof}

\input{multiplicative_interval_rules}

\begin{proof} ~
  \begin{enumerate}
    \item Claim $\ean[\epsilon]{a}\cdot \ean[\delta]{b} \subseteq \ean[\epsilon+\delta]{ab}$:

      \begin{align}
        x \in \ean[\epsilon]{a} \land y \in \ean[\delta]{b} & \implies \left(ae^{-\epsilon} \le x \le ae^{\epsilon}\right) \land \left(be^{-\delta} \le y \le be^\delta\right) \nl
        & \implies abe^{-(\epsilon+\delta)} \le xy \le abe^{\epsilon+\delta} \nl
        & \implies xy \in \ean[\epsilon+\delta]{a\cdot b}
      \end{align}

      Claim $\ean[\epsilon+\delta]{ab} \subseteq \ean[\epsilon]{a} \cdot \ean[\delta]{b}$: Let $f$ be the function $f: \ean[\epsilon]{a} \times \ean[\delta]{b} \to \R$ with $f(x,y) =xy$ so that $\ean[\epsilon]{a} \cdot \ean[\delta]{b}$ is the image of $f$. The function $f$ attains the maximum $abe^{\epsilon+\delta}$ of the interval $\ean[\epsilon+\delta]{ab}$ for $(x,y) = \left(ae^\epsilon,be^\delta\right)$ and its minimum $abe^{-(\epsilon+\delta)}$ for $(x,y)=\left(ae^{-\epsilon},be^{-\delta}\right)$. Because $f$ is continuous, $f$ attains each value between $abe^{-(\epsilon+\delta)}$ and $abe^{\epsilon+\delta}$ and therefore each value of $\ean[\epsilon+\delta]{ab}$ (intermediate value theorem~\cite{wiki:intermediatevaluetheorem}).

    \item

      \begin{align}
        \ean[\epsilon]{\ean[\delta]{a}} & = \bigcup_{x\in \ean[\delta]{a}} \ean[\epsilon]{x} = \bigcup_{x\in\ean[\epsilon]{a}} \bigcup_{y\in\ean[\epsilon]{1}} \{x\cdot y\} \nl
        &= \ean[\delta]{a} \cdot \ean[\epsilon]{1} = \ean[\epsilon+\delta]{a}
      \end{align}

    \item
      
      \begin{align}
        x\in\ean[\epsilon]{a} & \iff x \in \interval{ae^{-\epsilon}}{ae^\epsilon} \nl
        & \iff x \in \an[\frac{ae^\epsilon-ae^{-\epsilon}}2]{\frac{ae^\epsilon+ae^{-\epsilon}}2} \nl
        & \iff x \in \an[a\cdot \frac{e^\epsilon-e^{-\epsilon}}2]{a\cdot \frac{e^\epsilon+e^{-\epsilon}}2} \nl
        & \iff x\in \an[a\sinh(\epsilon)]{a\cosh(\epsilon)}
      \end{align}

    \item

      \begin{align}
        \ean[\epsilon]{a} &= \an[\sinh(\epsilon)a]{\cosh(\epsilon)a} \nl
        &= \an[\sinh(\epsilon)a]{a+\cosh(\epsilon)a-a} \nl
        &\subseteq \an[\sinh(\epsilon)a+\abs{\cosh(\epsilon)a-a}]{a} \nl
      &\begin{comment} a > 0 \land \cosh(\epsilon) > 0 \implies \cosh(\epsilon)a > a \end{comment} \nl
        &= \an[\sinh(\epsilon)a+\cosh(\epsilon)a-a]{a} \nl
      &\begin{comment} \sinh(\epsilon) + \cosh(\epsilon) = \frac 12 \left(e^\epsilon-e^{-\epsilon}\right) + \frac 12 \left(e^\epsilon+e^{-\epsilon}\right) = e^\epsilon \end{comment} \nl
        &= \an[e^\epsilon a-a]{a} \nl
        &= \an[\left(e^\epsilon-1\right)a]{a}
      \end{align}

    \item

      \begin{align}
        \abs{\frac ab - 1} \le \epsilon & \implies 1-\epsilon \le \frac ab \le 1+\epsilon \nl
        & \implies e^{-\epsilon} \le \frac ab \le e^{\epsilon} \nl
        & \implies be^{-\epsilon} \le a \le be^\epsilon \nl
        & \implies a \in \ean[\epsilon]{b}
      \end{align}
  \end{enumerate}

\end{proof}

\section{Big Psi notation}

\input{bigpsi_rules}

\begin{proof} ~
  \begin{enumerate}
    \item \label{proof:littleo_rule}

      \begin{align}
        & \seq{\epsilon_n}\in\bigo{a_n} \land \seq{a_n} \in \littleo{b_n} \nl
        \implies & \left(\exists C > 0: \limsup_{n\to\infty} \abs{\frac{\epsilon_n}{a_n}} \le C\right) \land \lim_{n\to\infty} \abs{\frac{a_n}{b_n}} = 0 \nl
        \implies & \lim_{n\to\infty} \abs{\frac{\epsilon_n}{b_n}} = \lim_{n\to\infty} \underbrace{\abs{\frac{\epsilon_n}{a_n}}}_{\text{bounded}} \cdot \underbrace{\abs{\frac{a_n}{b_n}}}_{\to 0} = 0 \nl
        \implies & \seq{\epsilon_n} \in \littleo{b_n}
      \end{align}
    \item

      \begin{align}
        \seq{\epsilon_n} \in \bigpsi{a_n} & \implies \limsup_{n\to\infty} \abs{\frac{\epsilon_n}{a_n}} \le 1 \nl
                                          & \implies \exists C_\infty > 0 : \limsup_{n\to\infty} \abs{\frac{\epsilon_n}{a_n}} \le C_\infty \nl
                                          & \implies \seq{e_n} \in \bigo{a_n}
      \end{align}

    \item

      \begin{align}
        & \seq{\epsilon_n} \in \bigpsi{a_n} \land \seq{\delta_n} \in \littleo{a_n} \nl
        \implies& \left(\limsup_{n\to\infty} \abs{\frac{\epsilon_n}{a_n}} \le 1\right) \land \left(\lim_{n\to\infty} \abs{\frac{\delta_n}{a_n}} = 0\right) \nl
        \implies& \limsup_{n\to\infty} \abs{\frac{\epsilon_n+\delta_n}{a_n}} \le \limsup_{n\to\infty} \left(\abs{\frac{\epsilon_n}{a_n}}+\abs{\frac{\delta_n}{a_n}}\right) \le 1 \nl
        \implies& \seq{\epsilon_n+\delta_n} \in \bigpsi{a_n}
      \end{align}

    \item

      \begin{align}
        \seq{\epsilon_n} \in \bigpsi{a_n}  & \implies \limsup_{n\to\infty} \abs{\frac{\epsilon_n}{a_n}} \le 1 \nl
        & \implies \limsup_{n\to\infty} \abs{\frac{\epsilon_n b_n}{a_n b_n}} = \limsup_{n\to\infty} \abs{\frac{\epsilon_n}{a_n}} \le 1 \nl
        & \implies \seq{\epsilon_n b_n} \in \bigpsi{a_n b_n}
      \end{align}

    \item

      \begin{align}
        \frac{\bigpsi{a_n}}{b_n} = \bigpsi{a_n} \cdot \frac{1}{b_n} \subseteq \bigpsi{\frac{a_n}{b_n}}
      \end{align}

    \item

      \begin{align}
        & \seq{\epsilon_n} \in \bigpsi{\lambda a_n} \land \seq{\delta_n} \in \bigpsi{\mu a_n} \nl
        \implies &
        \begin{aligned}
          \limsup_{n\to\infty} \abs{\frac{\epsilon_n+\delta_n}{(\lambda+\mu)a_n}} & \le \limsup_{n\to\infty} \left( \frac{\lambda}{\lambda + \mu} \cdot \underbrace{\abs{\frac{\epsilon_n}{\lambda a_n}}}_{\le 1} + \frac{\mu}{\lambda + \mu} \underbrace{\abs{\frac{\delta_n}{\mu a_n}}}_{\le 1} \right) \nl
          &\le \frac{\lambda}{\lambda+\mu} + \frac{\mu}{\lambda+\mu} = 1
        \end{aligned} \nl
        \implies & \seq{\epsilon_n+\delta_n} \in \bigpsi{(\lambda+\delta)a_n}
      \end{align}
    \item

      \begin{align}
        \seq{\epsilon_n} \in \littleo{1} & \implies \lim_{n\to\infty} \epsilon_n = 0 \nl
        & \implies \lim_{n\to\infty} e^{\epsilon_n} = 1 \nl
        & \implies \limsup_{n\to\infty} \frac{e^{\epsilon_n}}{1} \le 1 \nl
        & \implies \seq{e^{\epsilon_n}} \in \bigpsi{1}
      \end{align}

    \item

      Let $\seq{a_n}\in\littleo{1}$ and $\seq{\epsilon_n}\in\bigpsi{a_n}\subseteq \bigo{a_n}$. Rule \ref{proof:littleo_rule} implies $\seq{\epsilon_n} \in o(1)$ and thus $\lim_{n\to\infty} \epsilon_n = 0$. We have

      \begin{align}
        \limsup_{n\to\infty} \abs{\frac{e^{\epsilon_n}-1}{a_n}} = \limsup_{n\to\infty} \underbrace{\abs{\frac{e^{\epsilon_n}-1}{\epsilon_n}}}_{\to \exp'(0)=1} \cdot \underbrace{\abs{\frac{\epsilon_n}{a_n}}}_{\le 1} \le 1
      \end{align}

      \noindent Thus $\seq{e^{\epsilon_n}} \in \bigpsi{a_n}$.
  \end{enumerate}
\end{proof}
